wip: bumping Lawyer to work with newer Trillium

heap_lang/heap_lang_defs.v
@@ -1,71 +1,90 @@
-From iris.base_logic Require Export gen_heap.
+From iris.base_logic Require Export gen_heap. 
 From iris.proofmode Require Import tactics.
 From trillium.program_logic Require Export weakestpre.
 From heap_lang Require Export lang.
-From fairness Require Export execution_model.
+From trillium.program_logic Require Export execution_model iris_em.
 From heap_lang Require Import tactics notation.
 
 
-(* TODO: the missing fact of em_GS etc. being typeclasses
-   hardens automatic resolution of their instances *)
-Class heapGpreS Σ `(EM: ExecutionModel heap_lang M) := HeapPreG {
-  heapGpreS_inv :: invGpreS Σ;
+
+Class heap1GpreS Σ := HeapPreG {
+  (* heapGpreS_inv :: invGpreS Σ; *)
   heapGpreS_gen_heap :: gen_heapGpreS loc val Σ;
-  heapGpreS_em :: em_preGS Σ;
+  (* heapGpreS_em :: em_preGS Σ; *)
 }.
 
 
-Class heapGS Σ `(EM: ExecutionModel heap_lang M) := HeapG {
-  heap_inG :: heapGpreS Σ EM;
-
-  heap_invGS :: invGS_gen HasNoLc Σ;
+Class heap1GS Σ := HeapG {
+  heap_inG :: heap1GpreS Σ;
+  (* heap_invGS :: invGS_gen HasNoLc Σ; *)
   heap_gen_heapGS :: gen_heapGS loc val Σ;
-
-  heap_fairnessGS :: em_GS Σ;
+  (* heap_fairnessGS :: em_GS Σ; *)
 }.
 
-Definition heapΣ `(EM: ExecutionModel heap_lang M) : gFunctors :=
-  #[ invΣ; gen_heapΣ loc val; em_Σ ].
+Definition heap1Σ : gFunctors :=
+  #[ (* invΣ;  *)gen_heapΣ loc val  (* em_Σ *) ].
 
 
 (* TODO: automatize *)
-Global Instance subG_heapPreG {Σ} `{EM: ExecutionModel heap_lang M}:
-  subG (heapΣ EM) Σ → heapGpreS Σ EM.
-Proof. 
-  intros. 
-  enough (em_preGS Σ); [solve_inG| ].
-  apply em_Σ_subG. solve_inG.
-Qed. 
+Global Instance subG_heap1PreG {Σ}:
+  subG (heap1Σ) Σ → heap1GpreS Σ.
+Proof. solve_inG. Qed.
 
-#[global] Instance heapG_irisG `{EM: ExecutionModel heap_lang M} `{HGS: !heapGS Σ EM}:
-  irisG heap_lang M Σ := {
-    state_interp extr auxtr :=
-      (⌜em_valid_state_evolution_fairness extr auxtr⌝ ∗
-       gen_heap_interp (trace_last extr).2.(heap) ∗
-       em_msi (trace_last extr) (trace_last auxtr) (em_GS0 := heap_fairnessGS))%I ;
-    fork_post tid := fun _ => em_thread_post tid (em_GS0 := heap_fairnessGS);
+Global Instance HeapLangEM: LangEM heap_lang. 
+refine {| lgem_GS := heap1GS;
+          lgem_si `{heap1GS Σ} := fun c => gen_heap_interp (heap c);
+          lgem_init_resource `{heap1GS Σ} := fun c => ([∗ map] l↦v ∈ (heap c.2), pointsto l (DfracOwn 1) v)%I; |}. 
+- intros. eapply subG_heap1PreG. apply H.
+- simpl. intros Σ PRE c.
+  iMod (gen_heap_init c.2.(heap)) as (HEAP) "(HEAP & PTO & _)".
+  iModIntro. simpl. unshelve iExists _; [done| ].
+  iFrame.
+Defined.
+
+(** definitions to keep the existing proofs and TC inference working *)
+Class heapGpreS {Σ M} {EM: ExecutionModel heap_lang M} := {
+  heap_iemgPres :: @IEMGpreS _ _ HeapLangEM EM Σ;
+  heap_fairnessGpreS: em_preGS Σ := @iemGpreS_em _ _ _ _ _ heap_iemgPres;
 }.
+
+Class heapGS {Σ M} {EM: ExecutionModel heap_lang M} := {
+  heap_iemgs :: @IEMGS _ _ HeapLangEM EM Σ;
+  heap_fairnessGS: em_GS Σ := @iem_fairnessGS _ _ _ _ _ heap_iemgs;
+}.
+
+Global Instance heapPre_of_iemPre {Σ M} {EM: ExecutionModel heap_lang M}
+  (hGS: @heapGpreS Σ _ EM):
+  gen_heapGpreS loc val Σ.
+Proof using. apply hGS. Defined.
+
+Global Instance heap_of_iem {Σ M} {EM: ExecutionModel heap_lang M}
+  (hGS: @heapGS Σ _ EM):
+  gen_heapGS loc val Σ.
+Proof using. apply hGS. Defined.
+
 
 Section GeneralProperties.
   Context `{EM: ExecutionModel heap_lang M}. 
   Context `{HGS: @heapGS Σ _ EM}.
-  Let eGS := heap_fairnessGS. 
 
+  Existing Instance EM.
+  Let eGS := heap_fairnessGS.
+    
   Lemma posts_of_empty_mapping_multiple  (es e: expr) v (tid : nat) (tp : list expr):
     tp !! tid = Some e ->
     to_val e = Some v ->
     (* cur_posts tp e1 (fun _ => em_thread_post 0%nat (em_GS0 := eGS)) -∗ *)
-    (let Φs := map (fun τ _ => @em_thread_post heap_lang M EM Σ (@heap_fairnessGS Σ M EM _) τ) (seq 0 (length tp)) in
+    (let Φs := map (fun τ v => @em_thread_post heap_lang M EM Σ eGS τ v) (seq 0 (length tp)) in
       posts_of tp Φs) -∗
-    em_thread_post tid (em_GS0 := eGS).
+    em_thread_post tid v (em_GS0 := eGS).
   Proof.
     intros Hsome Hval. simpl.
     
-    rewrite (big_sepL_elem_of (λ x, x.2 x.1) _ (v, (fun _ => em_thread_post tid)) _) //.
+    rewrite (big_sepL_elem_of (λ x, x.2 x.1) _ (v, (fun v => em_thread_post tid v)) _) //.
     { eauto. } 
     apply elem_of_list_omap.
-    exists (e, (fun _ => em_thread_post tid (em_GS0 := eGS))); split; last first.
-    - simpl. apply fmap_Some. exists v. split; done.
+    exists (e, (fun v => em_thread_post tid v (em_GS0 := eGS))); split; last first.
+    - simpl. apply fmap_Some. exists v. split; done. 
     - destruct tp as [|e1' tp]; first set_solver. simpl.
       apply elem_of_cons.
       destruct tid as [|tid]; [left|right]; first by simpl in Hsome; simplify_eq.
@@ -82,16 +101,16 @@ Section GeneralProperties.
   Lemma posts_of_empty_mapping  (e1 e: expr) v (tid : nat) (tp : list expr):
     tp !! tid = Some e ->
     to_val e = Some v ->
-    cur_posts tp e1 (fun _ => em_thread_post 0%nat (em_GS0 := eGS)) -∗
-    em_thread_post tid (em_GS0 := eGS).
+    cur_posts tp e1 (fun (* τ  *) v => @em_thread_post heap_lang M EM Σ eGS 0%nat v) -∗
+    em_thread_post tid v (em_GS0 := eGS).
   Proof.
     intros Hsome Hval. simpl.
     
     rewrite /cur_posts. 
-    rewrite (big_sepL_elem_of (λ x, x.2 x.1) _ (v, (fun _ => em_thread_post tid)) _) //.
+    rewrite (big_sepL_elem_of (λ x, x.2 x.1) _ (v, (fun v => em_thread_post tid v)) _) //.
     { eauto. } 
     apply elem_of_list_omap.
-    exists (e, (fun _ => em_thread_post tid (em_GS0 := eGS))); split; last first.
+    exists (e, (fun v => em_thread_post tid v (em_GS0 := eGS))); split; last first.
     - simpl. apply fmap_Some. exists v. split; done.
     - destruct tp as [|e1' tp]; first set_solver. simpl.
       apply elem_of_cons.
