heap_lang/simulation_adequacy.v
@@ -1,175 +1,21 @@
 From stdpp Require Import fin_maps.
 From iris.proofmode Require Import tactics.
-From trillium.program_logic Require Export weakestpre adequacy.
-From fairness Require Export fairness traces_match trace_utils.
-From heap_lang Require Export lang heap_lang_defs.
+From trillium.traces Require Export traces_match trace_utils exec_traces.
+From trillium.program_logic Require Export weakestpre adequacy simulation_adequacy_em.
+From fairness Require Export fairness.
+From heap_lang Require Export heap_lang_defs lang.
+
 
 Definition heap_lang_extrace : Type := extrace heap_lang.
 
 
 Section adequacy.
 
-  Definition wp_premise
-    `{EM: ExecutionModel heap_lang M}
-    (Σ: gFunctors)
-    (s: stuckness) (e1 : expr) σ1 (s1: mstate M)
-    (R: execution_trace heap_lang → auxiliary_trace M → Prop)
-    (p: em_init_param)
-    := 
-    (∀ `{Hinv : @heapGS Σ M EM} ,
-        ⊢ (([∗ map] l ↦ v ∈ heap σ1, pointsto l (DfracOwn 1) v) ∗
-             em_init_resource s1 p (em_GS0 := heap_fairnessGS)
-           ={⊤}=∗
-              WP e1 @ s; locale_of [] e1; ⊤ {{ _, em_thread_post 0%nat (em_GS0 := heap_fairnessGS)}} ∗
-                                            rel_always_holds0 R s state_interp (fun _ => em_thread_post 0%nat (em_GS0 := heap_fairnessGS)) e1 σ1 s1)). 
-
-  Definition wp_premise_multiple
-    `{EM: ExecutionModel heap_lang M}
-    (Σ: gFunctors)
-    (s: stuckness) es σ1 (s1: mstate M)
-    (R: execution_trace heap_lang → auxiliary_trace M → Prop)
-    (p: em_init_param)
-    := 
-    (∀ `{Hinv : @heapGS Σ M EM} ,
-        ⊢ (([∗ map] l ↦ v ∈ heap σ1, pointsto l (DfracOwn 1) v) ∗
-             em_init_resource s1 p (em_GS0 := heap_fairnessGS)
-           ={⊤}=∗
-              let Φs := map (fun i _ => em_thread_post i%nat (em_GS0 := heap_fairnessGS)) (seq 0 (length es)) in
-              wptp s es Φs ∗
-              rel_always_holds s Φs R (es, σ1) s1)).
-
-  Lemma wp_premise_single `{EM: ExecutionModel heap_lang M} Σ
-    s e1 σ1 s1 R p:
-    wp_premise Σ s e1 σ1 s1 R p -> wp_premise_multiple Σ s [e1] σ1 s1 R p.
-  Proof using.
-    rewrite /wp_premise /wp_premise_multiple.
-    iIntros "%WP1 % [HEAP INIT]".
-    iMod (WP1 Hinv with "[$HEAP $INIT]") as "[WP1 RAH]".
-    iFrame. set_solver.
-  Qed.
-
-  Theorem strong_simulation_adequacy_general_multiple
-    `{hPre: @heapGpreS Σ M EM} (s: stuckness) (es : list expr) σ1 (s1: M)
-    (R: execution_trace heap_lang → auxiliary_trace M → Prop)
-    (p: em_init_param)    
-    :
-    length es ≥ 1 ->
-    rel_finitary R →
-    em_is_init_st (es, σ1) s1 ->
-    em_valid_state_evolution_fairness {tr[ (es, σ1) ]} {tr[ s1 ]} ->
-    (wp_premise_multiple Σ s es σ1 s1 R p) ->
-    continued_simulation R (trace_singleton (es, σ1)) (trace_singleton s1).
-  Proof.
-    intros LEN Hfin INIT VALID1 H.
-    apply (wp_strong_adequacy_multiple_with_trace_inv heap_lang M Σ s); try done.
-
-    iIntros (?) "".
-
-    iMod (gen_heap_init (heap σ1)) as (genheap)" [Hgen [Hσ _]]".  
-    iMod (em_initialization _ s1 (es, σ1) p) as (fGS) "[LM_INIT MSI]"; [done| ].
-    Unshelve. 2: by apply hPre. 
-
-    set (distG := {| heap_fairnessGS := (fGS: (em_GS Σ (ExecutionModel := EM))) |}).
-    iPoseProof (H distG) as "Hwp". clear H.
-    
-    iExists state_interp, (λ _ _, ⌜ True ⌝%I), _, (fun τ _ => em_thread_post τ).
-    iSplitR.
-    { unfold config_wp. iIntros "!>!>" (???????) "?". done. }
-
-    iSpecialize ("Hwp" with "[Hσ LM_INIT]"); [by iFrame| ]. 
-    iDestruct "Hwp" as ">[Hwp H]". 
-    iModIntro. iFrame "Hwp Hgen MSI".
-
-    (* TODO: make a lemma *)
-    iIntros (??????????) "SI POSTS".
-    rewrite /rel_always_holds. iDestruct ("H" with "[][][][][][][] SI POSTS") as "R".
-    all: try by done.
-    iSplit. 
-    - iModIntro; iIntros "[$ ?]"; done.
-    - eauto. 
-  Qed.
-
-  Theorem strong_simulation_adequacy_general
-    `{hPre: @heapGpreS Σ M EM} (s: stuckness) (e1 : expr) σ1 (s1: M)
-    (R: execution_trace heap_lang → auxiliary_trace M → Prop)
-    (p: em_init_param)
-    :
-    rel_finitary R →
-    em_is_init_st ([e1], σ1) s1 ->
-    em_valid_state_evolution_fairness {tr[ ([e1], σ1) ]} {tr[ s1 ]} ->
-    (wp_premise Σ s e1 σ1 s1 R p) ->
-    continued_simulation R (trace_singleton ([e1], σ1)) (trace_singleton s1).
-  Proof.
-    intros. eapply strong_simulation_adequacy_general_multiple.
-    1-4: by eauto.
-    apply wp_premise_single. eauto. 
-  Qed.
-
-  Theorem strong_simulation_adequacy_inftraces_multiple Σ
-    `{hPre: @heapGpreS Σ M EM} (s: stuckness) 
-    (es : list expr) σ1 (s1: M)
-    (R: execution_trace heap_lang → auxiliary_trace M → Prop)
-    (p: em_init_param)
-    (iex : inf_execution_trace heap_lang)
-    (Hvex : valid_inf_exec (trace_singleton (es, σ1)) iex)
-    :
-    length es ≥ 1 ->
-    rel_finitary R →
-    em_is_init_st (es, σ1) s1 ->
-    (wp_premise_multiple Σ s es σ1 s1 R p) ->
-    exists iatr,
-      @valid_inf_system_trace _ M
-        (@continued_simulation
-           heap_lang
-           M
-           R)
-        (trace_singleton (es, σ1))
-        (trace_singleton s1)
-        iex
-        iatr.
-  Proof.
-    intros LEN Hfin Hwp.
-    eexists.
-    eapply produced_inf_aux_trace_valid_inf.
-    Unshelve.
-    - econstructor.
-    - eapply (strong_simulation_adequacy_general_multiple s) => //.
-    - done.
-  Qed.
-
-  Theorem strong_simulation_adequacy_inftraces Σ
-    `{hPre: @heapGpreS Σ M EM} (s: stuckness) 
-    (e1 : expr) σ1 (s1: M)
-    (R: execution_trace heap_lang → auxiliary_trace M → Prop)
-    (p: em_init_param)
-    (iex : inf_execution_trace heap_lang)
-    (Hvex : valid_inf_exec (trace_singleton ([e1], σ1)) iex)
-    :
-    rel_finitary R →
-    em_is_init_st ([e1], σ1) s1 ->
-    (wp_premise Σ s e1 σ1 s1 R p) ->
-    exists iatr,
-      @valid_inf_system_trace _ M
-        (@continued_simulation
-           heap_lang
-           M
-           R)
-        (trace_singleton ([e1], σ1))
-        (trace_singleton s1)
-        iex
-        iatr.
-  Proof.
-    intros. eapply strong_simulation_adequacy_inftraces_multiple.
-    1-5: by eauto.
-    by eapply wp_premise_single. 
-  Qed.
-
-  Theorem strong_simulation_adequacy_traces_multiple Σ
+  Theorem strong_simulation_adequacy_traces_multiple_HL Σ
     `{hPre: @heapGpreS Σ M EM} (s: stuckness) 
     (es: list expr) σ1 (s1: M)
     (R: execution_trace heap_lang → auxiliary_trace M → Prop)
     (p: em_init_param)
-
     (extr : heap_lang_extrace)
     (Hvex : extrace_valid extr)
     (Hexfirst : trfirst extr = (es, σ1))
@@ -191,97 +37,47 @@ Section adequacy.
     length es ≥ 1 ->
     rel_finitary R →
     em_is_init_st (es, σ1) s1 ->
-    (wp_premise_multiple Σ s es σ1 s1 R p) ->
+    (wp_premise_multiple R Σ s es σ1 s1 p) ->
     ∃ (mtr : trace (mstate M) (mlabel M)), 
       traces_match lbl_rel state_rel locale_step (@mtrans M) extr mtr /\
       trfirst mtr = s1. 
-  Proof.
-    intros ? Hfin INIT Hwp.
-    have [iatr MATCH] : exists iatr,
-        @valid_inf_system_trace
-          heap_lang M
-          (@continued_simulation
-             heap_lang
-             M
-             R)
-          (trace_singleton (es, (trfirst extr).2))
-          (trace_singleton s1)
-          (from_trace extr)
-          iatr.
-    { eapply (strong_simulation_adequacy_inftraces_multiple _ s); eauto.
-      1: eapply from_trace_preserves_validity; eauto; first econstructor.
-      all: try by rewrite Hexfirst. }
-    rewrite Hexfirst in MATCH. simpl in *. 
-    exists (to_trace s1 iatr).
-
-    split.
-    2: { by rewrite to_trace_trfirst. }
-
-    pose proof MATCH as INF_REF. (** see remark below *)
-    eapply (valid_inf_system_trace_implies_traces_match
-                       valid_step                       
-                       state_rel
-                       lbl_rel
-                       ltac:(idtac)
-                       ltac:(idtac)
-                       (continued_simulation R)) in MATCH; cycle 1.  
-    { intros ?? ?%continued_simulation_rel. eauto. }
-    { intros ?? ?%continued_simulation_rel. eauto. }
-    { apply from_trace_spec. simpl.
-      rewrite Hexfirst. done. }
-    { apply to_trace_spec. }
-    Unshelve. 2,3: by eauto.
-    
-    assert (exists len, trace_len.trace_len_is extr len /\ trace_len.trace_len_is (to_trace s1 iatr) len) as LEN. (** see remark below *)
-    { simpl in MATCH.
-      pose proof (trace_len.trace_has_len extr) as [len LEN]. 
-      pose proof (trace_len.trace_has_len (to_trace s1 iatr)) as [len' LEN'].
-      eapply trace_len.traces_match_same_length in MATCH; eauto. subst.  
-      eauto. }
-
-    (** INF_REF and LEN together give the traces mentioned in
-        the refinement section of Lawyer paper
-        (same length, related by infinite extension of refinement).       
-        However, our proofs proceed differency, 
-        using the notion of traces_match (MATCH hypothesis). *)
-
-    apply MATCH. 
+  Proof using.
+    intros. eapply strong_simulation_adequacy_traces_multiple; eauto.
+    esplit; try by (apply _ || apply hPre). 
   Qed.
 
-  Theorem strong_simulation_adequacy_traces Σ
-    `{hPre: @heapGpreS Σ M EM} (s: stuckness) 
-    (e1 : expr) σ1 (s1: M)
-    (R: execution_trace heap_lang → auxiliary_trace M → Prop)
-    (p: em_init_param)
+  (* Theorem strong_simulation_adequacy_traces Σ *)
+  (*   `{hPre: @heapGpreS Σ M EM} (s: stuckness)  *)
+  (*   (e1 : expr) σ1 (s1: M) *)
+  (*   (R: execution_trace heap_lang → auxiliary_trace M → Prop) *)
+  (*   (p: em_init_param) *)
 
-    (extr : heap_lang_extrace)
-    (Hvex : extrace_valid extr)
-    (Hexfirst : trfirst extr = ([e1], σ1))
+  (*   (extr : heap_lang_extrace) *)
+  (*   (Hvex : extrace_valid extr) *)
+  (*   (Hexfirst : trfirst extr = ([e1], σ1)) *)
 
-    (valid_step: cfg heap_lang -> olocale heap_lang → cfg heap_lang → 
-                 mstate M → mlabel M → mstate M -> Prop)
-    (state_rel: cfg heap_lang -> mstate M -> Prop)
-    (lbl_rel: olocale heap_lang -> mlabel M -> Prop)
-    (STEP_LBL_REL: forall c1 oζ c2 δ1 ℓ δ2,
-                 valid_step c1 oζ c2 δ1 ℓ δ2 ->
-                 lbl_rel oζ ℓ)
-    (STEP_MTRANS: forall c1 oζ c2 δ1 ℓ δ2,
-                 valid_step c1 oζ c2 δ1 ℓ δ2 ->
-                 mtrans δ1 ℓ δ2)
-    (R_ST: forall extr mtr, R extr mtr -> state_rel (trace_last extr) (trace_last mtr))
-    (R_STEP: forall extr mtr, R extr mtr -> valid_state_evolution_fairness valid_step extr mtr)
+  (*   (valid_step: cfg heap_lang -> olocale heap_lang → cfg heap_lang →  *)
+  (*                mstate M → mlabel M → mstate M -> Prop) *)
+  (*   (state_rel: cfg heap_lang -> mstate M -> Prop) *)
+  (*   (lbl_rel: olocale heap_lang -> mlabel M -> Prop) *)
+  (*   (STEP_LBL_REL: forall c1 oζ c2 δ1 ℓ δ2, *)
+  (*                valid_step c1 oζ c2 δ1 ℓ δ2 -> *)
+  (*                lbl_rel oζ ℓ) *)
+  (*   (STEP_MTRANS: forall c1 oζ c2 δ1 ℓ δ2, *)
+  (*                valid_step c1 oζ c2 δ1 ℓ δ2 -> *)
+  (*                mtrans δ1 ℓ δ2) *)
+  (*   (R_ST: forall extr mtr, R extr mtr -> state_rel (trace_last extr) (trace_last mtr)) *)
+  (*   (R_STEP: forall extr mtr, R extr mtr -> valid_state_evolution_fairness valid_step extr mtr) *)
 
-    :
-    rel_finitary R →
-    em_is_init_st ([e1], σ1) s1 ->
-    (wp_premise Σ s e1 σ1 s1 R p) ->
-    ∃ (mtr : trace (mstate M) (mlabel M)), 
-      traces_match lbl_rel state_rel locale_step (@mtrans M) extr mtr /\
-      trfirst mtr = s1. 
-  Proof.
-    intros. eapply strong_simulation_adequacy_traces_multiple; last first.
-    { by eapply wp_premise_single. }
-    all: by eauto.     
-  Qed.
+  (*   : *)
+  (*   rel_finitary R → *)
+  (*   em_is_init_st ([e1], σ1) s1 -> *)
+  (*   (wp_premise Σ s e1 σ1 s1 R p) -> *)
+  (*   ∃ (mtr : trace (mstate M) (mlabel M)),  *)
+  (*     traces_match lbl_rel state_rel locale_step (@mtrans M) extr mtr /\ *)
+  (*     trfirst mtr = s1.  *)
+  (* Proof. *)
+  (*   foobar.  *)
+  (* Qed. *)
   
 End adequacy.
