lawyer/obligations/env_helpers.v
@@ -24,7 +24,7 @@ Global Existing Instance om_hl_LvlO_equiv.
 Class OM_HL_Env `(OP: OP_HL DegO LvlO LIM_STEPS)
   `(EM: ExecutionModel heap_lang M) (Σ: gFunctors):= {
     ohe_oGS' : @asem_GS _ _ ObligationsASEM Σ;
-    ohe_hGS :: heapGS Σ EM;
+    ohe_hGS :: @heapGS _ _ EM;
 
     ohe_obls_AMU : @AMU_lift_MU _ _ _ ohe_oGS' _ EM ohe_hGS (↑ nroot);
     ohe_obls_AMU__f : forall τ, @AMU_lift_MU__f _ _ _ τ ohe_oGS' _ EM _ ⊤;
